@prefix bibo: <http://purl.org/ontology/bibo/> .
@prefix lv:   <http://purl.org/lobid/lv#> .
@prefix rdf:  <http://www.w3.org/1999/02/22-rdf-syntax-ns#> .
@prefix owl:  <http://www.w3.org/2002/07/owl#> .
@prefix dct:  <http://purl.org/dc/terms/> .
@prefix bf: <http://id.loc.gov/ontologies/bibframe/> .
@prefix rdfs: <http://www.w3.org/2000/01/rdf-schema#> .
@prefix foaf: <http://xmlns.com/foaf/0.1/> .
@prefix oo: <http://purl.org/openorg/> .
@prefix schema: <http://schema.org/> .
@prefix skos: <http://www.w3.org/2004/02/skos/core#> .
@prefix vann: <http://purl.org/vocab/vann/> .
@prefix voaf: <http://purl.org/vocommons/voaf#> .
@prefix vs: <http://www.w3.org/2003/06/sw-vocab-status/ns#> .
@prefix xsd: <http://www.w3.org/2001/XMLSchema#> .

# About lobid vocab

<http://purl.org/lobid/lv>
   rdf:type owl:Ontology , voaf:Vocabulary ;
   vann:preferredNamespacePrefix "lv" ;
   dct:title "lobid vocab" ;
   dct:license <http://creativecommons.org/publicdomain/zero/1.0/> ;
   dct:description "Under this name space new properties and classes needed for the service lobid ('linking open bibliographic data') are defined . Already existing properties and classes which are (re)used in lobid aren't documented here."@en ;
   dct:issued "2012-01-17" ;
   dct:modified "2024-02-16"^^xsd:date ;
   skos:historyNote "See the commit history for this vocabulary at https://github.com/lobid/vocabs/commits/master/lobid-vocab.ttl." ;
   dct:publisher <http://lobid.org/organisation/DE-605> ;
   dct:creator <http://lobid.org/team/ap> ;
   vann:preferredNamespaceUri "http://purl.org/lobid/lv#" ;
   oo:contact <mailto:semweb@hbz-nrw.de> .


# <http://purl.org/lobid/lv#ArchivedWebPage>

lv:ArchivedWebPage
   a owl:Class ;
   rdfs:subClassOf <http://data.archiveshub.ac.uk/def/ArchivalResource> , bf:Archival ;
   rdfs:label "Archived Web Page"@en ;
   rdfs:label "Archivierte Webseite"@de ;
   rdfs:isDefinedBy <http://purl.org/lobid/lv> ;
   rdfs:comment "An archival resource that is product of archiving a web page."@en ;
   rdfs:comment "Das Produkt der Archivierung einer Webseite."@de .

# <http://purl.org/lobid/lv#BibliographicDescription>

lv:BibliographicDescription
   a owl:Class ;
   rdfs:subClassOf bibo:Document ;
   rdfs:label "Bibliographic description"@en ;
   rdfs:label "Bibliographische Beschreibung"@de ;
   rdfs:isDefinedBy <http://purl.org/lobid/lv> ;
   rdfs:comment "A description of a bibliographic resource, e.g. in form of a metadata record."@en , "Die Beschreibung einer bibliographischen Ressource, z.B. in Form eines Metadatensatzes."@de .

# <http://purl.org/lobid/lv#Bibliography>

lv:Bibliography
   a owl:Class ;
   rdfs:subClassOf bibo:Collection ;
   rdfs:label "Bibliography"@en ;
   rdfs:label "Bibliografie"@de ;
   rdfs:isDefinedBy <http://purl.org/lobid/lv> ;
   rdfs:comment "A collection of documents relevant to a particular subject or author."@en ;
   rdfs:comment "Eine Sammlung von Literaturnachweisen."@de .


# <http://purl.org/lobid/lv#Biography>

lv:Biography
   a owl:Class ;
   rdfs:subClassOf dct:BibliographicResource ;
   rdfs:label "Biography"@en ;
   rdfs:label "Biografie"@de ;
   rdfs:isDefinedBy <http://purl.org/lobid/lv> ;
   rdfs:comment "A detailed description or account of a person's life"@en ;
   rdfs:comment "Die Lebensbeschreibung einer Person."@de .


# <http://purl.org/lobid/lv#EditedVolume>

lv:EditedVolume
   a owl:Class ;
   rdfs:subClassOf bibo:Collection ;
   rdfs:label "Edited Volume"@en ;
   rdfs:label "Aufsatzsammlung"@de ;
   rdfs:isDefinedBy <http://purl.org/lobid/lv> ;
   rdfs:comment "a collection of scholarly or scientific articles written by different authors"@en ;
   rdfs:comment "Ein Sammelwerk mit mehreren Beiträgen."@de .


# <http://purl.org/lobid/lv#Festschrift>

lv:Festschrift
   a owl:Class ;
   rdfs:subClassOf dct:BibliographicResource ;
   rdfs:label "Festschrift"@en ;
   rdfs:label "Festschrift"@de ;
   rdfs:isDefinedBy <http://purl.org/lobid/lv> ;
   rdfs:comment "A publication honoring a respected person, especially an academic."@en ;
   rdfs:comment "Einem Gelehrten gewidmete Sammlung von Aufsätzen."@de .


# <http://purl.org/lobid/lv#IsPartOfRelation>

lv:IsPartOfRelation
   a owl:Class ;
   rdfs:label "Part-of relation"@en ;
   rdfs:label "Teil-von-Beziehung"@de ;
   rdfs:isDefinedBy <http://purl.org/lobid/lv> ;
   rdfs:comment "The relationship between a resource and a superordinate resource it is part of."@en ;
   rdfs:comment "Die Beziehung zwischen einer Ressource und der ihr übergeordneten Ressource."@de .


# <http://purl.org/lobid/lv#Miscellaneous>

lv:Miscellaneous
   a owl:Class ;
   rdfs:subClassOf dct:BibliographicResource ;
   rdfs:label "Miscellaneous"@en ;
   rdfs:label "Sonstige"@de ;
   rdfs:isDefinedBy <http://purl.org/lobid/lv> ;
   rdfs:comment "This class covers all publication types that are not covered by existing class definitions. It is used to enable facets over seldomly found publication types in library catalogs."@en ;
   rdfs:comment "Diese Klasse deckt alle Publikationstypen ab, die nicht durch bestehende Klassen erfasst sind. Sie dient insbesondere dem Angebot von Facetten für jene Publikationstypen, die in Bibliothekskatalogen selten zu finden sind."@de ;
   rdfs:seeAlso <https://wiki1.hbz-nrw.de/x/E4AyAQ#Facettenueberhbz01-Daten-misc> .


# <http://purl.org/lobid/lv#MultiVolumeWorkRelation>

lv:MultiVolumeWorkRelation
   a owl:Class ;
   rdfs:label "Volume-to-work relation"@en ;
   rdfs:label "Band-Werk-Beziehung"@de ;
   rdfs:isDefinedBy <http://purl.org/lobid/lv> ;
   rdfs:comment "The relationship between a volume and a multi-volume work it is part of."@en ;
   rdfs:comment "Die Beziehung zwischen einem Band und dem übergeordneten mehrbändigen Werk."@de .


# <http://purl.org/lobid/lv#OfficialPublication>

lv:OfficialPublication
   a owl:Class ;
   rdfs:subClassOf dct:BibliographicResource ;
   rdfs:label "Official Publication"@en ;
   rdfs:label "Amtliche Veröffentlichung"@de ;
   rdfs:isDefinedBy <http://purl.org/lobid/lv> ;
   rdfs:comment "A publication that records the business and proceedings of a government agency."@en ;
   rdfs:comment "Eine behördliche Publikation für amtliche Bekanntmachungen."@de .


# <http://purl.org/lobid/lv#Schoolbook>

lv:Schoolbook
   a owl:Class ;
   rdfs:subClassOf dct:BibliographicResource ;
   rdfs:label "Schoolbook"@en ;
   rdfs:label "Schulbuch"@de ;
   rdfs:isDefinedBy <http://purl.org/lobid/lv> ;
   rdfs:comment "A textbook used by school teachers in their classes."@en ;
   rdfs:comment "Ein Lehrbuch, das Schullehrer im Unterricht einsetzen."@de .


# <http://purl.org/lobid/lv#SecondaryPublicationEvent>

lv:SecondaryPublicationEvent
   a owl:Class ;
   rdfs:subClassOf schema:PublicationEvent ;
   rdfs:label "Publication Event of Secondary Form"@en ;
   rdfs:label "Publikation der Sekundärform"@de ;
   rdfs:isDefinedBy <http://purl.org/lobid/lv> ;
   rdfs:comment "The publication event of a reproduction/secondary form of an already published work (e.g. digitised media or microform)."@en ;
   rdfs:comment "Das Ereignis der Publikation einer Reproduktion/Sekundärform (z.B. Digitalisat oder Mikroform)."@de .


# <http://purl.org/lobid/lv#SeriesRelation>

lv:SeriesRelation
   a owl:Class ;
   rdfs:label "Resource-to-series relation"@en ;
   rdfs:label "Dokument-Reihe-Beziehung"@de ;
   rdfs:isDefinedBy <http://purl.org/lobid/lv> ;
   rdfs:comment "The relationship between a resource and a series it is part of."@en ;
   rdfs:comment "Die Beziehung zwischen einem Dokument und einer Reihe."@de .


# <http://purl.org/lobid/lv#Statistics>

lv:Statistics
   a owl:Class ;
   rdfs:subClassOf dct:BibliographicResource ;
   rdfs:label "Statistics"@en ;
   rdfs:label "Statistik"@de ;
   rdfs:isDefinedBy <http://purl.org/lobid/lv> ;
   rdfs:comment "A systematic collection and analysis of empirical data."@en ;
   rdfs:comment "Eine systematische Sammlung und Analyse von empirischen Daten."@de .


# <http://purl.org/lobid/lv#ags>

lv:ags
   rdf:type owl:DatatypeProperty ;
   rdfs:label "Amtlicher Gemeindeschlüssel"@de ;
   rdfs:label "Community Identification Number"@en ;
   rdfs:isDefinedBy <http://purl.org/lobid/lv> ;
   rdfs:comment "Amtlicher Gemeindeschlüssel (AGS) of the region a spatial resource is located in."@en ;
   rdfs:comment "Amtlicher Gemeindeschlüssel (AGS) der Region, in der sich die beschriebene raum-zeitliche Ressource befindet."@de ;
   rdfs:seeAlso <http://de.wikipedia.org/wiki/Amtlicher_Gemeindeschl%C3%BCssel> , <http://en.wikipedia.org/wiki/Community_Identification_Number#Germany> ;
   rdfs:range xsd:positiveInteger .


# <http://purl.org/lobid/lv#almaMmsId>

lv:almaMmsId
   rdf:type owl:DatatypeProperty ;
   rdfs:label "Alma MMS ID"@de ;
   rdfs:label "Alma MMS ID"@en ;
   rdfs:isDefinedBy <http://purl.org/lobid/lv> ;
   rdfs:comment "Die Datensatz-ID im Alma Metadata Management System (MMS). Die MMS ID kann 8 bis 19 Stellen land sein (wobei die ersten beiden Stellen den Datensatztyp angeben und die letzten vier Stellen auf den Identifikator für die Institution bezug nehmen.)"@de ;
   rdfs:comment "The record ID number in the Alma Metadata Management System (MMS). The MMS ID can be 8 to 19 digits long (with the first two digits referring to the record type and the last four digits referring to a unique identifier for the institution)."@en ;
   rdfs:subPropertyOf dct:identifier ;
   rdfs:domain dct:BibliographicResource ;
   rdfs:range rdfs:Literal .


# <http://purl.org/lobid/lv#bibliographicLevel>

lv:bibliographicLevel
   rdf:type owl:DatatypeProperty ;
   rdfs:label "Bibliografisches Level"@de ;
   rdfs:label "Bibliographic Level"@en ;
   rdfs:isDefinedBy <http://purl.org/lobid/lv> ;
   rdfs:comment "Beschreibt das bibliografische Level einer Ressource, angeleht an MARC 21-Leader 07 - Bibliographic level: https://www.loc.gov/marc/bibliographic/bdleader.html"@de ;
   rdfs:comment "Describes the bibliographic level of a resource, based on MARC 21-Leader 07 -  - Bibliographic level: https://www.loc.gov/marc/bibliographic/bdleader.html"@en ;
   rdfs:domain dct:BibliographicResource ;
   rdfs:range rdfs:Literal .


# <http://purl.org/lobid/lv#callNumber>

lv:callNumber
    a owl:DatatypeProperty ;
    rdfs:comment "A call number, shelf mark or other identifier for an item"@en ;
    rdfs:domain bf:Item;
    rdfs:label "call number"@en ;
    rdfs:label "Signatur"@de ;
    rdfs:isDefinedBy <http://purl.org/lobid/lv> ;
    rdfs:range rdfs:Literal ;
    rdfs:subPropertyOf dct:identifier .


# <http://purl.org/lobid/lv#currentLocation>

lv:currentLocation
    a owl:DatatypeProperty ;
    rdfs:comment "The location of an item"@en ;
    rdfs:domain bf:Item;
    rdfs:label "current location"@en ;
    rdfs:label "Standort"@de ;
    rdfs:isDefinedBy <http://purl.org/lobid/lv> ;
    rdfs:range rdfs:Literal .

# <http://purl.org/lobid/lv#currentLibrary>

lv:currentLibrary
    a owl:DatatypeProperty ;
    rdfs:comment "The specific library within an institution holding an item"@en ;
    rdfs:domain bf:Item;
    rdfs:label "current location"@en ;
    rdfs:label "Standort"@de ;
    rdfs:isDefinedBy <http://purl.org/lobid/lv> ;
    rdfs:range rdfs:Literal .

# <http://purl.org/lobid/lv#contactqr>

lv:contactqr
   rdf:type owl:ObjectProperty ;
   owl:deprecated true ;
   rdfs:label "Contact QR code"@en ;
   rdfs:label "Kontakt-QR-Code"@de ;
   rdfs:isDefinedBy <http://purl.org/lobid/lv> ;
   rdfs:comment "Relates a person, organization or other agent to a QR code that encodes the agent's contact information."@en ;
   rdfs:domain foaf:Agent ;
   rdfs:range foaf:Image .


# <http://purl.org/lobid/lv#containedIn>

lv:containedIn
   rdf:type owl:ObjectProperty ;
   rdfs:label "Contained in"@en ;
   rdfs:label "Enthalten in"@de ;
   rdfs:isDefinedBy <http://purl.org/lobid/lv> ;
   rdfs:comment "This property is used to link an article to a journal or an edited volume it is contained in."@en ;
   rdfs:comment "Diese Property verlinkt einen Artikel mit einer Zeitschrift oder einer Aufsatzsammlung, in der er enthalten ist."@de;
   rdfs:subPropertyOf dct:isPartOf;
   rdfs:domain bibo:BibliographicResource ;
   rdfs:range dct:BibliographicResource .


# <http://purl.org/lobid/lv#containsExampleOfWork>

lv:containsExampleOfWork
   rdf:type owl:ObjectProperty ;
   rdfs:label "Contains example of work"@en ;
   rdfs:label "Enthält eine Instanz des Werkes"@de ;
   rdfs:isDefinedBy <http://purl.org/lobid/lv> ;
   rdfs:comment "This property is used to indicate a work of which the resource contains an instance. Traditionally, this work is identified by a uniform title and optionally with a GND ID."@en ;
   rdfs:comment "Diese Property verweist auf ein Werk, von dem die Ressource eine Instanz beinhaltet. Das heißt, hier werden Einheitssachtitel und optional die GND-ID eines Werks angegeben, von dem die Ressource eine Instanz enthält."@de;
   rdfs:domain bibo:BibliographicResource ;
   rdfs:range <http://d-nb.info/standards/elementset/gnd#Work> .

[ ] rdfs:subPropertyOf lv:containsExampleOfWork ;
   owl:propertyChainAxiom (
   bf:hasPart
   bf:instanceOf
   ) .

[ ] rdfs:subPropertyOf lv:containsExampleOfWork ;
   owl:propertyChainAxiom (
   schema:hasPart
   schema:exampleOfWork
   ) .


# <http://purl.org/lobid/lv#dbsID>

lv:dbsID
   rdf:type owl:DatatypeProperty ;
   rdfs:label "DBS-ID"@de ;
   rdfs:label "DBS ID"@en ;
   rdfs:isDefinedBy <http://purl.org/lobid/lv> ;
   rdfs:comment "DBS-Nummer. Der Identifier, der einer Bibliothek innerhalb der Deutschen Bibliotheksstatistik (DBS) zugewiesen wurde."@de ;
   rdfs:comment "The identifier that was assigned to a library in the context of the German Library Statistics (DBS)."@en ;
   rdfs:subPropertyOf dct:identifier ;
   rdfs:domain schema:Library ;
   rdfs:range rdfs:Literal .


# <http://purl.org/lobid/lv#dnbID>

lv:dnbID
   rdf:type owl:DatatypeProperty ;
   rdfs:label "DNB-ID"@de ;
   rdfs:label "DNB ID"@en ;
   rdfs:isDefinedBy <http://purl.org/lobid/lv> ;
   rdfs:comment "DNB-Nummer. Der Identifier, der einer bibliographischen Ressource im Katalog der DNB (Deutsche National Bibliothek) zugewiesen wurde."@de ;
   rdfs:comment "The identifier that is assigned to a bibliographic resource in the catalogue of the German National Library (DNB, Deutsche National Bibliothek))."@en ;
   rdfs:subPropertyOf dct:identifier ;
   rdfs:domain dct:BibliographicResource ;
   rdfs:range rdfs:Literal .


# <http://purl.org/lobid/lv#fulltextOnline>

lv:fulltextOnline
   rdf:type owl:ObjectProperty ;
   rdfs:label "Fulltext online"@en ;
   rdfs:label "Online-Volltext"@de ;
   rdfs:isDefinedBy <http://purl.org/lobid/lv> ;
   rdfs:comment "Relates a bibliographic resource to an online resource (full text in HTML, PDFs or landing pages in OA repositories, on publishers' websites etc.) that represents the full text of the bibliographic resource or contains a link to a full text of the resource. "@en ;
   rdfs:domain dct:BibliographicResource ;
   rdfs:range foaf:Document .


# <http://purl.org/lobid/lv#fundertype>

lv:fundertype
   rdf:type owl:ObjectProperty ;
   rdfs:label "Type of funding organization"@en ;
   rdfs:label "Art des Unterhaltträgers"@de ;
   rdfs:isDefinedBy <http://purl.org/lobid/lv> ;
   rdfs:comment "Indicates which type an institution's funder is of. It should be used with a controlled vocabulary like http://purl.org/lobid/fundertype."@en ;
   rdfs:domain foaf:Organization ;
   rdfs:range skos:Concept .


# <http://purl.org/lobid/lv#hasSuperordinate>

lv:hasSuperordinate
  rdf:type owl:ObjectProperty ;
  rdfs:label "Übergeordnete Ressource"@en ;
  rdfs:label "Superordinate resource"@de ;
  rdfs:isDefinedBy <http://purl.org/lobid/lv> ;
  rdfs:comment "This property is used to link a is-part-of relation to a superordinate resource."@en ;
  rdfs:comment "Diese Property verlinkt eine Teil-von-Beziehung mit der übergeordneten Ressource."@de;
  rdfs:domain lv:IsPartRelation ;
  rdfs:range dct:BibliographicResource .

[ ] rdfs:subPropertyOf dct:isPartOf ;
  owl:propertyChainAxiom (
  lv:isPartOf
  lv:hasSuperordinate
  ) .


# <http://purl.org/lobid/lv#hbzID>

lv:hbzID
   rdf:type owl:DatatypeProperty ;
   rdfs:label "hbz-ID"@de ;
   rdfs:label "hbz ID"@en ;
   rdfs:isDefinedBy <http://purl.org/lobid/lv> ;
   rdfs:comment "HT-Nummer. Der Identifier, der einer bibliographischen Ressource im hbz-Verbundkatalog zugewiesen wurde."@de ;
   rdfs:comment "The identifier that is assigned to a bibliographic resource in the hbz union catalogue."@en ;
   rdfs:subPropertyOf dct:identifier ;
   rdfs:domain dct:BibliographicResource ;
   rdfs:range rdfs:Literal .


# <http://purl.org/lobid/lv#inCollection>

lv:inCollection
   rdf:type owl:ObjectProperty ;
   rdfs:label "in collection"@en ;
   rdfs:label "In Sammlung"@de ;
   rdfs:isDefinedBy <http://purl.org/lobid/lv> ;
   rdfs:comment "This property is used to link a bibliographic resource to a collection (bibliography, repository etc.) it is part of."@en ;
   rdfs:comment "Diese Property verlinkt eine Ressource mit einer Sammlung (Bibliographie, Dokumentenserver etc.), zu der sie gehört."@de;
   rdfs:domain dct:BibliographicResource .


# <http://purl.org/lobid/lv#inDataset>

   lv:inDataset
      rdf:type owl:ObjectProperty ;
      rdfs:label "in data set"@en ;
      rdfs:label "In Dataset"@de ;
      rdfs:isDefinedBy <http://purl.org/lobid/lv> ;
      rdfs:comment "This property is used to link a data record to a data set it is part of."@en ;
      rdfs:comment "Diese Property verlinkt einen Datensatz mit einem Dataset, zu dem er gehört."@de;
      rdfs:range schema:Dataset .


# <http://purl.org/lobid/lv#inSeries>

lv:inSeries
   rdf:type owl:ObjectProperty ;
   rdfs:label "in series"@en ;
   rdfs:label "In Reihe"@de ;
   rdfs:isDefinedBy <http://purl.org/lobid/lv> ;
   rdfs:comment "This property is used to link a document to a document-to-series relation."@en ;
   rdfs:comment "Diese Property verlinkt eine Ressource mit einer Dokument-Serie-Beziehung."@de;
   rdfs:domain dct:BibliographicResource ;
   rdfs:range lv:SeriesRelation .


# <http://purl.org/lobid/lv#inventoryNumber>

lv:inventoryNumber
    a owl:DatatypeProperty ;
    rdfs:comment "An inventoryNumber for an item different to call number and shelf mark"@en ;
    rdfs:domain bf:Item;
    rdfs:label "inventory number"@en ;
    rdfs:label "Inventarnummer"@de ;
    rdfs:isDefinedBy <http://purl.org/lobid/lv> ;
    rdfs:range rdfs:Literal ;
    rdfs:subPropertyOf dct:identifier .

# <http://purl.org/lobid/lv#isil>

lv:isil
   rdf:type owl:DatatypeProperty ;
   rdfs:label "ISIL" ;
   rdfs:isDefinedBy <http://purl.org/lobid/lv> ;
   rdfs:comment "International Standard Identifier for Libraries and Related Organizations (ISIL). Ein eindeutiger Identifikator für Bibliotheken und verwandte Einrichtungen oder untergeordnete Organisationseinheiten, der durch ISIL-Agenturen vergeben wird. Das Literal sollte durch den folgenden regulären Ausdruck gematcht werden: [A-Z]{1,4}-[0-9a-zA-Z:-/]{1,11} ."@de ;
   rdfs:comment "International Standard Identifier for Libraries and Related Organizations (ISIL). 'An ISIL identifies an organization, i.e., a library or a related organization, or one of its subordinate units, which is responsible for an action or service in a bibliographic environment (e.g. creation of machine-readable information). It can be used to identify the originator or holder of a resource (e.g. library material).' The literal should conform to this regular expression: [A-Z]{1,4}-[0-9a-zA-Z:-/]{1,11} ."@en ;
   rdfs:subPropertyOf dct:identifier ;
   rdfs:seeAlso <http://biblstandard.dk/isil/scope.htm> ;
   rdfs:range [
      a rdfs:Datatype ;
      owl:onDatatype xsd:string ;
      owl:withRestrictions (
        [
            xsd:pattern "[A-Z]{1,4}-[0-9a-zA-Z:-/]{1,11}"
        ]
      )
              ]  .


# <http://purl.org/lobid/lv#isPartOf>

lv:isPartOf
    rdf:type owl:ObjectProperty ;
    rdfs:label "is part of"@en ;
    rdfs:label "Bestandteil von"@de ;
    rdfs:isDefinedBy <http://purl.org/lobid/lv> ;
    rdfs:comment "This property is used to link a resource to a is-part-of relation."@en ;
    rdfs:comment "Diese Property verlinkt eine Ressource mit einer Teil-von-Beziehung."@de;
    rdfs:domain dct:BibliographicResource ;
    rdfs:range lv:IsPartOfRelation .


# <http://purl.org/lobid/lv#manufacture>

lv:manufacture
   rdf:type owl:DatatypeProperty ;
   rdfs:label "Manufacture"@en ;
   rdfs:label "Herstellung"@de ;
   rdfs:isDefinedBy <http://purl.org/lobid/lv> ;
   rdfs:comment "This property is used to state manufacture information."@en ;
   rdfs:range rdfs:Literal .


# <http://purl.org/lobid/lv#manufacturedBy>

lv:manufacturedBy
   rdf:type owl:DatatypeProperty ;
   rdfs:label "Manufactured by"@en ;
   rdfs:label "Hergestellt durch"@de ;
   rdfs:isDefinedBy <http://purl.org/lobid/lv> ;
   rdfs:comment "This property is used to state the manufactureres."@en ;
   rdfs:range rdfs:Literal .


# <http://purl.org/lobid/lv#multiVolumeWork>

lv:multiVolumeWork
   rdf:type owl:ObjectProperty ;
   rdfs:label "Multi-volume work"@en ;
   rdfs:label "Mehrbändiges Werk"@de ;
   rdfs:isDefinedBy <http://purl.org/lobid/lv> ;
   rdfs:comment "This properties is used to link a volume-to-work relation to a volume."@en ;
   rdfs:comment "Diese Property verlinkt eine Band-Werk-Beziehung mit einem mehrbändigen Werk."@de;
   rdfs:domain lv:MultiVolumeWorkRelation ;
   rdfs:range dct:BibliographicResource .


# <http://purl.org/lobid/lv#numbering>

lv:numbering
   rdf:type owl:ObjectProperty ;
   rdfs:label "numbering"@en ;
   rdfs:label "Nummer"@de ;
   rdfs:isDefinedBy <http://purl.org/lobid/lv> ;
   rdfs:comment "This property is used to indicate the numbering within a volume-to-work or a document-to-series relation."@en ;
   rdfs:comment "Zur Angabe der Nummerierung innerhalb einer Band-Werk-Beziehung oder Dokument-Reihe-Beziehung."@de;
   rdfs:domain [ a owl:Class;
        owl:unionOf (  lv:MultiVolumeWorkRelation lv:SeriesRelation)
    ];
   rdfs:range rdfs:Literal .

# <http://purl.org/lobid/lv#nwbibsubject>

lv:nwbibsubject
   rdf:type owl:ObjectProperty ;
   rdfs:label "NWBib-Sachschlagwort"@de ;
   rdfs:label "NWBib subject heading"@en ;
   rdfs:isDefinedBy <http://purl.org/lobid/lv> ;
   rdfs:comment "Verlinkt eine Ressource aus der Nordrhein-Westfälischen Bibliographie (NWBib) mit einer Systemstelle aus der NWBib-Sachsystematik (http://purl.org/lobid/nwbib)."@de ;
   rdfs:comment "Links a resource in the Northrhine-Westphalian Bibliography (NWBib) to a concept in NWBib's subject classification (http://purl.org/lobid/nwbib)."@en ;
   rdfs:subPropertyOf dct:subject ;
   rdfs:domain dct:BibliographicResource ;
   rdfs:range skos:Concept ;
   vs:status "deprecated" .


# <http://purl.org/lobid/lv#nwbibspatial>

lv:nwbibspatial
   rdf:type owl:ObjectProperty ;
   rdfs:label "NWBib-Ortsschlagwort"@de ;
   rdfs:label "NWBib spatial subject heading"@en ;
   rdfs:isDefinedBy <http://purl.org/lobid/lv> ;
   rdfs:comment "Verlinkt eine Ressource aus der Nordrhein-Westfälischen Bibliographie mit einer Systemstelle aus der NWBib-Ortssystematik (http://purl.org/lobid/nwbib-spatial)."@de ;
   rdfs:comment "Links a resource in the Northrhine-Westphalian Bibliography (NWBib) to a concept in NWBib's spatial classification (http://purl.org/lobid/nwbib-spatial)."@en ;
   rdfs:subPropertyOf dct:subject ;
   rdfs:domain dct:BibliographicResource ;
   rdfs:range skos:Concept ;
   vs:status "deprecated" .


# <http://purl.org/lobid/lv#rpbSubject>

lv:rpbSubject
   rdf:type owl:ObjectProperty ;
   rdfs:label "RPB-Sachschlagwort"@de ;
   rdfs:label "RPB subject heading"@en ;
   rdfs:isDefinedBy <http://purl.org/lobid/lv> ;
   rdfs:comment "Verlinkt eine Ressource aus der Rheinland-Pfälzischen Bibliographie (RPB) mit einer Systemstelle aus einer RPB-Sachsystematik: http://purl.org/lobid/rpb und https://w3id.org/lobid/rpb2."@de ;
   rdfs:comment "Links a resource in the Bibliography of Rhineland-Palatinate (RPB) to a concept in one of RPB's subject classification: http://purl.org/lobid/rpb and https://w3id.org/lobid/rpb2."@en ;
   rdfs:subPropertyOf dct:subject ;
   rdfs:domain dct:BibliographicResource ;
   rdfs:range skos:Concept ;
   vs:status "deprecated" .


# <http://purl.org/lobid/lv#rs>

lv:rs
   rdf:type owl:DatatypeProperty ;
   rdfs:label "Regionalschlüssel"@de ;
   rdfs:label "Region key"@en ;
   rdfs:isDefinedBy <http://purl.org/lobid/lv> ;
   rdfs:comment "Key of the region a spatial resource is located in."@en ;
   rdfs:comment "Regionalschlüssel der Region, in der sich die beschriebene raum-zeitliche Ressource befindet."@de ;
   rdfs:seeAlso <https://de.wikipedia.org/wiki/Amtlicher_Gemeindeschl%C3%BCssel#Regionalschl.C3.BCssel> ;
   rdfs:range xsd:positiveInteger .

# <http://purl.org/lobid/lv#series>

lv:series
   rdf:type owl:ObjectProperty ;
   rdfs:label "Series"@en ;
   rdfs:label "Reihe"@de ;
   rdfs:isDefinedBy <http://purl.org/lobid/lv> ;
   rdfs:comment "This property is used to link a document-to-series relation to a series."@en ;
   rdfs:comment "Diese Property verlinkt eine Dokument-Serie-Beziehung mit einer Serie."@de;
   rdfs:domain lv:SeriesRelation ;
   rdfs:range dct:BibliographicResource .


# <http://purl.org/lobid/lv#sigel>

lv:sigel
   rdf:type owl:DatatypeProperty ;
   rdfs:label "Sigel" ;
   rdfs:isDefinedBy <http://purl.org/lobid/lv> ;
   rdfs:comment "Ein eindeutiger Identifikator für D-A-CH Bibliotheken, der durch Sigel-Agenturen vergeben wird."@de ;
   rdfs:comment "Unique identifier for libraries from Germany, Austria and Switzerland, assigned by the Sigil-Agency."@en ;
   rdfs:subPropertyOf dct:identifier ;
   rdfs:seeAlso <https://sigel.staatsbibliothek-berlin.de/vergabe/sigel> ;
   rdfs:range rdfs:Literal .

# <http://purl.org/lobid/lv#stockNumber>

lv:stockNumber
   rdf:type owl:DatatypeProperty ;
   rdfs:label "Publisher or Distributor Number"@en ;
   rdfs:label "Verlags-/Vertriebsnummer"@de ;
   rdfs:isDefinedBy <http://purl.org/lobid/lv> ;
   rdfs:comment "States the publisher or distributor number of a resource, based on MARC 21-028 - Publisher or Distributor Number: https://www.loc.gov/marc/bibliographic/bd028.html"@en ;
   rdfs:domain dct:BibliographicResource ;
   rdfs:range rdfs:Literal .


# <http://purl.org/lobid/lv#stocksize>

lv:stocksize
   rdf:type rdf:Property ;
   owl:deprecated true ;
   rdfs:label "Stock Size"@en ;
   rdfs:label "Bestandsgröße"@de ;
   rdfs:isDefinedBy <http://purl.org/lobid/lv> ;
   rdfs:comment "Indicates an institution's stock size. This property is especially used to indicate the size of a library's collection. It is recommended to be used with the controlled vocabulary at http://purl.org/lobid/stocksize."@en ;
   rdfs:domain foaf:Organization .


# <http://purl.org/lobid/lv#subjectChain>

lv:subjectChain
   rdf:type owl:DatatypeProperty ;
   rdfs:label "Chain of subject terms"@en ;
   rdfs:label "Schlagwortfolge"@de ;
   rdfs:isDefinedBy <http://purl.org/lobid/lv> ;
   rdfs:comment "A pipe-separated list of subject terms, optionally followed by a comma-seperated list of permutations (in parentheses)."@en ;
   rdfs:domain dct:BibliographicResource ;
   rdfs:range rdfs:Literal ;
   vs:status "deprecated" .


# <http://purl.org/lobid/lv#subjectAltLabel>

lv:subjectAltLabel
   rdf:type rdf:Property ;
   rdfs:label "Variant spelling of a subject heading"@en ;
   rdfs:label "Abweichende Benennung eines Schlagworts"@de ;
   rdfs:isDefinedBy <http://purl.org/lobid/lv> ;
   rdfs:comment "Contains labels which are used for search but are not shown in the frontend."@en ;
   rdfs:domain dct:BibliographicResource ;
   rdfs:range rdfs:Literal .


# <http://purl.org/lobid/lv#titleKeyword>

lv:titleKeyword
   rdf:type owl:DatatypeProperty ;
   rdfs:label "Title keyword"@en ;
   rdfs:label "Titelstichwort"@de ;
   rdfs:isDefinedBy <http://purl.org/lobid/lv> ;
   rdfs:comment "Indicates a title keyword, possibly in a different spelling than used in the original title."@en ;
   rdfs:domain schema:CreativeWork .


# <http://purl.org/lobid/lv#urn>

lv:urn
   rdf:type owl:DatatypeProperty ;
   rdfs:label "URN"@en ;
   rdfs:label "URN"@de ;
   rdfs:isDefinedBy <http://purl.org/lobid/lv> ;
   rdfs:comment "This property is used to indicate the uniform resource name (URN) of a bibliographic resource. The URN must be stated as a string not as URI, thus identifying the identifier itself and not the resource that is identified by the URN."@en ;
   rdfs:domain dct:BibliographicResource ;
   rdfs:range rdfs:Literal .


# <http://purl.org/lobid/lv#volumeIn>

lv:volumeIn
   rdf:type owl:ObjectProperty ;
   rdfs:label "volume in"@en ;
   rdfs:label "Bestandteil von"@de ;
   rdfs:isDefinedBy <http://purl.org/lobid/lv> ;
   rdfs:comment "This property is used to link a volume to a volume-to-work relation."@en ;
   rdfs:comment "Diese Property verlinkt ein Band mit einer Band-Werk-Beziehung."@de;
   rdfs:domain dct:BibliographicResource ;
   rdfs:range lv:MultiVolumeWorkRelation .


# <http://purl.org/lobid/lv#webPageArchived>

lv:webPageArchived
   rdf:type owl:ObjectProperty ;
   rdfs:label "Web page archived"@en ;
   rdfs:label "Archivierte Webseite"@de ;
   rdfs:isDefinedBy <http://purl.org/lobid/lv> ;
   rdfs:comment "This property is used to link the product of archiving a web page to the web page being archived."@en ;
   rdfs:domain lv:ArchivedWebPage ;
   rdfs:range schema:WebPage .


# <http://purl.org/lobid/lv#zdbID>

lv:zdbID
   rdf:type owl:DatatypeProperty ;
   rdfs:label "ZDB-ID"@de ;
   rdfs:label "ZDB ID"@en ;
   rdfs:isDefinedBy <http://purl.org/lobid/lv> ;
   rdfs:comment "ZDB-Nummer. Der Identifier, der einer bibliographischen Ressource in der Zeitschriftendatenbank (ZDB) zugewiesen wurde."@de ;
   rdfs:comment "The identifier that is assigned to a bibliographic resource in the German Journal Database (Zeitschriftendatenbank, ZDB)."@en ;
   rdfs:subPropertyOf dct:identifier ;
   rdfs:domain dct:BibliographicResource ;
   rdfs:range rdfs:Literal .
